more imp loop ideas

CPS_Ctl/ImpCtl.thy
@@ -67,7 +67,10 @@ definition imp_ctl_sem :: "syn' \<Rightarrow> 'x imp_state' \<Rightarrow> 'x imp
         (case l of
          [cond, body] \<Rightarrow> cond # (G z [cond, cond, body]) # t
          | [cond, _, body] \<Rightarrow> (if b then body # (G z [cond, body]) # t else t)
-         | _ \<Rightarrow> [] \<comment> \<open> error \<close>))
+         | _ \<Rightarrow> [] \<comment> \<open> error \<close>)
+        | SwhileC \<Rightarrow>
+        (case l of [body] \<Rightarrow> (if b then body # (G z [body]) # t else t)
+         | _ \<Rightarrow> []))
       , b))"
 
 (*
@@ -594,6 +597,211 @@ next
 qed
 *)
 
+lemma rtranclp_induct_alt :
+  assumes H : "rtranclp r a b" 
+  assumes Ha : "P a" 
+  assumes Hsteps : "(\<And> y z . rtranclp r a y \<Longrightarrow> rtranclp r y z \<Longrightarrow> P y \<Longrightarrow> P z)" 
+  shows "P b" using assms
+proof(induction rule: rtranclp_induct)
+  case base
+  then show ?case by auto
+next
+  case (step y z)
+
+  have Py : "P y" using step.IH[OF step.prems(1) step.prems(2)]
+    by auto
+
+  have Rz : "rtranclp r y z" using step.hyps
+    by(auto)
+
+  show ?case using step.prems(2)[OF step.hyps(1) Rz Py] by auto
+qed
+
+(*
+lemma rtranclp_induct_alt_stronger :
+  "rtranclp r a b \<Longrightarrow> P a \<Longrightarrow>
+   (\<And> y z . rtranclp r a y \<Longrightarrow> rtranclp r y z \<Longrightarrow> P y \<Longrightarrow> P z) \<Longrightarrow> P b"
+proof(induction rule: rtranclp_induct)
+  case base
+  then show ?case by auto
+next
+  case (step y z)
+
+  have Py : "P y" using step.IH[OF step.prems(1) step.prems(2)]
+    by auto
+
+  have Rz : "rtranclp r y z" using step.hyps
+    by(auto)
+
+  show ?case using step.prems(2)[OF step.hyps(1) Rz Py] by auto
+qed
+*)
+
+(* the issue here is that we don't really have any way of describing what might happen after
+executing a prefix before the loop, since that prefix might do all kinds of crazy stuff
+to the continuation
+
+*)
+
+(*
+lemma HWhile_gen :
+  assumes H0 : "gs = \<lparr> s_sem = pcomps' fs \<rparr>"
+  (*assumes H1 : "seq_sem_l_gen lfts \<in> set fs" *)
+  assumes HF : "f = imp_sem_l_gen lfts"
+  assumes Hpres : "sups_pres (set fs)"
+  assumes Hnemp : "g \<in> set fs"
+  assumes Hdom : "(f \<downharpoonleft> (set fs) Swhile')"
+  assumes Hsyn : "lfts Swhile' = Swhile"
+  (* TODO: generalize. these should be expressed using valid-sets *)
+  assumes P1_valid : "\<And> st.  P1 st \<Longrightarrow> get_cond st \<noteq> None"
+  assumes P2_valid : "\<And> st.  P2 st \<Longrightarrow> get_cond st \<noteq> None"
+  assumes Hcond : "|gs| {- P1 -} [cond] {- P1 -}"
+  assumes Htrue : "|gs| {- (\<lambda> st . P1 st \<and> get_cond st = Some True) -} [body]
+                        {- P1 -}"
+(*
+  assumes Hfalse : "\<And> st . P2 st \<and> get_cond st = Some False \<Longrightarrow> P1 st" 
+*)
+  shows "|gs| {- P1 -} [G Swhile' [cond, body]] {- (\<lambda> st . P1 st ) -}"
+proof-
+
+*)
+
+(* proof sketch idea: need to show that we don't crash after n steps.
+   0 steps easy, we start with a valid continuation
+
+we took n steps. wlog we are in thhe body somewhere.
+*)
+
+lemma HWhileC_gen :
+  assumes H0 : "gs = \<lparr> s_sem = pcomps' fs \<rparr>"
+  (*assumes H1 : "seq_sem_l_gen lfts \<in> set fs" *)
+  assumes HF : "f = imp_sem_l_gen lfts"
+  assumes Hpres : "sups_pres (set fs)"
+  assumes Hnemp : "g \<in> set fs"
+  assumes Hdom : "(f \<downharpoonleft> (set fs) SwhileC')"
+  assumes Hsyn : "lfts Swhile' = SwhileC"
+  (* TODO: generalize. these should be expressed using valid-sets *)
+  assumes PX_valid : "\<And> n st.  PX n st \<Longrightarrow> get_cond st \<noteq> None"
+  assumes Htrue : "\<And> n . |gs| {-(\<lambda> st . PX n st)-} [body] {-(\<lambda> st . PX (n + 1) st)-}"
+  assumes PX_P1 : "\<And> n st . PX n st \<Longrightarrow> P1 st"
+  assumes PX_P1' : "\<And> st . P1 st \<Longrightarrow> PX 0 st"
+  shows "|gs| {- PX mz  -} [G SwhileC' [body]] {- (\<lambda> st . (\<exists> n . PX (mz + n) st \<and> get_cond st = Some False) ) -}"
+proof
+  fix c'
+  assume Guard : "|gs| {\<lambda>st. \<exists>n. PX (mz + n) st \<and> get_cond st = Some False} c'"
+
+  show "|gs| {PX mz} [G SwhileC' [body]] @ c'"
+  proof
+    fix m :: "('a, 'b) state"
+
+    assume M : "PX mz (payload m)"
+    assume CM : "s_cont m = Inl ([G SwhileC' [body]] @ c')"
+
+    show "(safe gs m)"
+    proof(cases "(sem_step gs m)")
+      case (Inr bad)
+
+      then have False using CM H0
+        by(auto simp add: sem_step_def)
+
+      then show ?thesis by auto
+    next
+      case (Inl m')
+
+      have F_eq : "sem_step \<lparr> s_sem = f \<rparr> m = Inl m'"
+        using sym[OF dominant_pcomps'[OF Hpres Hnemp Hdom]] CM Inl H0
+        by(simp add: sem_step_def)
+
+      have M_P1 : "PX mz (payload m)" using PX_P1' M by auto
+
+      have M'_valid : "\<And> p . fst (payload m) \<noteq> mdp p None" using PX_valid[OF M_P1]
+        by(auto simp add: get_cond_def split:prod.splits)
+
+      have Sm' : "payload m = payload m'"
+        using CM Hsyn F_eq M'_valid  unfolding HF
+        by(cases m; cases m'; auto simp add: s_cont_def sem_step_def imp_sem_l_gen_def imp_ctl_sem_def imp_sem_lifting_gen_def
+           schem_lift_defs 
+          merge_l_def fst_l_def snd_l_def prio_l_def triv_l_def option_l_def LNew_def
+          split: md_prio.splits md_triv.splits option.splits)
+
+      have M' : "PX mz (payload m')" using Sm' M_P1 by auto
+
+      show "safe gs m" using HTE[OF Htrue]
+      proof(cases "\<exists>n st. PX n (payload st) \<and> get_cond (payload st) = Some False")
+        case True
+        then show ?thesis sorry
+      next
+        case False
+
+        then have "\<And> n st . PX n (payload st) \<Longrightarrow> get_cond (payload st) = Some True"
+          sorry
+
+        show ?thesis
+        proof
+          fix mfin
+          assume "sem_exec_p gs m mfin"
+          show "imm_safe gs mfin"
+      qed
+
+      show "safe gs m" using guardedD[OF Guard]
+      proof(cases "get_cond (payload m)")
+        case None
+
+        then have False using PX_valid[OF M_P1]
+          by(auto simp add: get_cond_def split: prod.splits md_prio.splits md_triv.splits option.splits)
+        then show ?thesis by auto
+
+      next
+        case Some' : (Some cnd)
+        then show ?thesis 
+        proof(cases cnd)
+          case True
+    
+          have Mp2'_cond : "get_cond (payload m') = Some True" 
+            using CM Hsyn H0 M' F_eq PX_valid[OF M_P1] True Some' unfolding HF
+            by(cases m; cases m'; 
+                auto simp add: s_cont_def sem_step_def imp_sem_l_gen_def imp_ctl_sem_def imp_sem_lifting_gen_def
+                schem_lift_defs 
+                merge_l_def fst_l_def snd_l_def prio_l_def triv_l_def option_l_def LNew_def
+                get_cond_def
+                split: md_prio.splits md_triv.splits option.splits)
+
+          have Mp2'_p2_true :  "PX 0 (payload m') \<and> get_cond (payload m') = Some True"
+            using M' Mp2'_cond
+            by auto
+
+          have Mp2'_cont : "s_cont m' = Inl ([body, G SwhileC' [body]] @ c')" sorry
+(*
+            using  Hsyn H0 MP1 F_eq' P1_valid[OF MP1] True Some' unfolding HF
+            by(cases mp2; cases mp2'; 
+                auto simp add: s_cont_def sem_step_def imp_sem_l_gen_def imp_ctl_sem_def imp_sem_lifting_gen_def
+                schem_lift_defs 
+                merge_l_def fst_l_def snd_l_def prio_l_def triv_l_def option_l_def LNew_def
+                get_cond_def
+                split: md_prio.splits md_triv.splits option.splits)
+*)
+
+
+          have Mp2'_safe : "safe gs m'"
+          proof
+            fix m''
+
+            assume H'' : "sem_exec_p gs m' m''"
+
+
+            then obtain n where N : "sem_exec_c_p gs m' n m''" sorry
+
+            then show "imm_safe gs m''"
+            proof(induction rule: sem_exec_c_p.induct)
+            case (Excp_0 m)
+              then show ?case sorry
+            next
+              case (Excp_Suc m1 m2 n m3)
+              then show ?case 
+            qed
+
+
+(*
 lemma HWhile_gen :
   assumes H0 : "gs = \<lparr> s_sem = pcomps' fs \<rparr>"
   (*assumes H1 : "seq_sem_l_gen lfts \<in> set fs" *)
@@ -630,19 +838,256 @@ proof
   have Gtrue' : "|gs| {\<lambda>st. P1 st \<and> get_cond st = Some True} [body, cond] @ c'"
     using HTE[OF Htrue Gcond] by auto
 
-  have Test : "\<And> c' . 
-|gs| {\<lambda> st . P1 st \<and> get_cond st = Some True}  [body, G Swhile' [cond, body]]  @ c' \<Longrightarrow>
-|gs| { P1 } [cond, G Swhile' [cond, cond, body]] @ c' \<Longrightarrow>
-|gs| {P1} ([G Swhile' [cond, body]] @ c')"
+(*
+  have Gtrue_real : "|gs| {-\<lambda> st. P1 st \<and> get_cond st = Some True-} [body, G Swhile' [cond, body]] {-P1-}"
   proof
-    fix c' 
+    fix c''
+
+    assume Hc'' : "|gs| {P1} c''"
+
+    show "|gs| {\<lambda>st. P1 st \<and>
+                      get_cond st =
+                      Some True} [body, G Swhile' [cond, body]] @ c''"
+    proof
+      fix m :: "('a, 'b) state"
+
+      assume K0 : "P1 (payload m) \<and> get_cond (payload m) = Some True"
+      assume K1 : "s_cont m = Inl ([body, G Swhile' [cond, body]] @ c'')"
+
+      obtain x1 x2 where Body : "G x1 x2 = body"
+        by(cases body; auto)
+
+
+      have "\<And> m' b . sem_exec_p gs m m' \<Longrightarrow> s_cont m' = Inr b \<Longrightarrow> False"
+      proof-
+        fix m' b
+        assume Xc : "sem_exec_p gs m m'"
+        assume Cn : "s_cont m' = Inr b"
+
+(* we need something along the lines of "no-cheating" -
+   need to be able to say that if 
+   m is safe for cont = Inl ([body, G Swhile' [cond, body]] @ c''
+   then it must also be safe for [body] (or vice versa?)
+*)
+
+        show False using HCat[OF Htrue]
+          sorry
+      qed
+(*
+      show "safe gs m"
+      proof
+        fix m' :: "('a, 'b) state"
+
+        assume Xp : "sem_exec_p gs m m'" 
+        show "imm_safe gs m'"
+*)
+      show "safe gs m"
+      proof(rule safe_for_safe; rule safe_forI)
+        fix n n' :: nat
+        fix m' :: "('a, 'b) state"
+
+        assume N: "n' < n"
+        assume M' : "sem_exec_c_p gs m n' m'"
+        show "imm_safe gs m'"
+          using M' N K0 K1
+        proof(induction n arbitrary: m m')
+          case 0
+          then show ?case by auto
+        next
+          case (Suc nx)
+
+          then obtain m'1 where M'1 : "sem_step gs m = Inl m'1"
+            unfolding sem_step_def using Body K1
+            by(cases "sem.s_sem gs x1 m"; auto)
+
+          then show ?case using HCat
+        qed
+          case (Excp_0 m)
+  
+          then have "(\<exists>m'. sem_step gs m = Inl m')"
+            unfolding sem_step_def using Body 
+            by(cases "sem.s_sem gs x1 m"; auto)
+  
+          then show ?case unfolding imm_safe_def sem_step_p_eq
+            by auto
+        next
+          case (Excp_Suc m1 m2 nx m3)
+          then show ?case 
+        qed
+          case base
+          then show ?case 
+        next
+          case (step y z)
+          then show ?case sorry
+        qed
+
+  have Gtrue_real : "|gs| {\<lambda> st . P1 st \<and> get_cond st = Some True} [body, G Swhile' [cond, body]] @ c'"
+  proof
     fix m :: "('a, 'b) state"
 
-    assume A0 : "|gs| {\<lambda> m . P1 m \<and> get_cond m = Some True} [body, G Swhile' [cond, body]] @ c'"
-    assume A1 : "|gs| {P1} [cond, G Swhile' [cond, cond, body]] @ c'"
-    assume Pay : "P1 (payload m)"
-    assume Cont : "s_cont m = 
-      Inl ([G Swhile' [cond, body]] @ c')"
+    assume Hm1 : "P1 (payload m) \<and> get_cond (payload m) = Some True"
+    assume Hm2 : "s_cont m = Inl ([body, G Swhile' [cond, body]] @ c')"
+    show "safe gs m"
+    proof
+      fix m'
+      assume Hm' : "sem_exec_p gs m m'"
+      show "imm_safe gs m'" using Hm' Hm1 Hm2 unfolding sem_exec_p_def
+      proof(induction arbitrary: c' rule: converse_rtranclp_induct)
+        case base
+        show ?case using guardedD[OF Gtrue ] base.prems
+      next
+        case (step y z)
+        then show ?case sorry
+      qed
+*)
+  show "|gs| {P1} [G Swhile' [cond, body]] @ c'"
+  proof
+
+    fix m :: "('a, 'b) state"
+
+    assume M : "P1 (payload m)"
+    assume CM : "s_cont m = Inl ([G Swhile' [cond, body]] @ c')"
+
+    show "safe gs m"
+    proof(cases "(sem_step gs m)")
+      case (Inr bad)
+
+      then have False using CM H0
+        by(auto simp add: sem_step_def)
+
+      then show ?thesis by auto
+    next
+      case (Inl m')
+
+      have F_eq : "sem_step \<lparr> s_sem = f \<rparr> m = Inl m'"
+        using sym[OF dominant_pcomps'[OF Hpres Hnemp Hdom]] CM Inl H0
+        by(simp add: sem_step_def)
+
+      have CM' : "s_cont m' = Inl ([cond] @ ([ G Swhile' [cond, cond, body]] @ c'))" 
+        using CM Hsyn F_eq unfolding HF
+        by(cases m; cases m'; auto simp add: s_cont_def sem_step_def imp_sem_l_gen_def imp_ctl_sem_def imp_sem_lifting_gen_def
+           schem_lift_defs 
+          merge_l_def fst_l_def snd_l_def prio_l_def triv_l_def option_l_def
+          split: md_prio.splits md_triv.splits option.splits)
+
+      have M'_valid : "\<And> p . fst (payload m) \<noteq> mdp p None" using P1_valid[OF M]
+        by(auto simp add: get_cond_def split:prod.splits)
+
+      have Sm' : "payload m = payload m'"
+        using CM Hsyn F_eq M'_valid  unfolding HF
+        by(cases m; cases m'; auto simp add: s_cont_def sem_step_def imp_sem_l_gen_def imp_ctl_sem_def imp_sem_lifting_gen_def
+           schem_lift_defs 
+          merge_l_def fst_l_def snd_l_def prio_l_def triv_l_def option_l_def LNew_def
+          split: md_prio.splits md_triv.splits option.splits)
+
+      hence P1sm' : "P1 (payload m')" using M unfolding Sm' by auto
+
+      (* next: step to the end of cond. *)
+
+      have Sub : "|gs| {P1} [G Swhile' [cond, cond, body]] @ c'"
+      proof
+        fix mp2 :: "('a, 'b) state"
+
+        assume MP2 : "P1 (payload mp2)"
+
+        assume Cont2 : "s_cont mp2 = Inl ([G Swhile' [cond, cond, body]] @ c')"
+
+        show "safe gs mp2"
+        proof(cases "get_cond (payload mp2)")
+          case None
+
+          then have False using P1_valid[OF MP2]
+            by(auto simp add: get_cond_def split: prod.splits md_prio.splits md_triv.splits option.splits)
+          then show ?thesis by auto
+
+        next
+          case Some' : (Some cnd)
+          then show ?thesis 
+          proof(cases "sem_step gs mp2")
+            case (Inr bad)
+
+            then have False using Cont2 H0
+              by(auto simp add: sem_step_def)
+
+            then show ?thesis by auto
+
+          next
+            case (Inl mp2')
+
+            have F_eq' : "sem_step \<lparr> s_sem = f \<rparr> mp2 = Inl mp2'"
+              using sym[OF dominant_pcomps'[OF Hpres Hnemp Hdom]] Cont2 Inl H0
+              by(simp add: sem_step_def)
+
+            have Mp2'_p2 : "P1 (payload mp2')"
+              using Cont2 Hsyn H0 MP2 F_eq' P1_valid[OF MP2] Some' unfolding HF
+              by(cases mp2; cases mp2'; 
+                  auto simp add: s_cont_def sem_step_def imp_sem_l_gen_def imp_ctl_sem_def imp_sem_lifting_gen_def
+                  schem_lift_defs 
+                  merge_l_def fst_l_def snd_l_def prio_l_def triv_l_def option_l_def LNew_def
+                  get_cond_def
+                  split: md_prio.splits md_triv.splits option.splits)
+
+            show ?thesis
+            proof(cases cnd)
+              case True
+
+              have Mp2'_cond : "get_cond (payload mp2') = Some True" 
+                using Cont2 Hsyn H0 MP2 F_eq' P1_valid[OF MP2] True Some' unfolding HF
+                by(cases mp2; cases mp2'; 
+                    auto simp add: s_cont_def sem_step_def imp_sem_l_gen_def imp_ctl_sem_def imp_sem_lifting_gen_def
+                    schem_lift_defs 
+                    merge_l_def fst_l_def snd_l_def prio_l_def triv_l_def option_l_def LNew_def
+                    get_cond_def
+                    split: md_prio.splits md_triv.splits option.splits)
+
+              have Mp2'_p2_true :  "P1 (payload mp2') \<and> get_cond (payload mp2') = Some True"
+                using Mp2'_p2 Mp2'_cond
+                by auto
+
+              have Mp2'_cont : "s_cont mp2' = Inl ([body] @ [G Swhile' [cond, body]] @ c')"
+                using Cont2 Hsyn H0 MP2 F_eq' P1_valid[OF MP2] True Some' unfolding HF
+                by(cases mp2; cases mp2'; 
+                    auto simp add: s_cont_def sem_step_def imp_sem_l_gen_def imp_ctl_sem_def imp_sem_lifting_gen_def
+                    schem_lift_defs 
+                    merge_l_def fst_l_def snd_l_def prio_l_def triv_l_def option_l_def LNew_def
+                    get_cond_def
+                    split: md_prio.splits md_triv.splits option.splits)
+
+              have Mp2'_safe : "safe gs mp2'"
+                using guardedD[OF Gtrue ] Mp2'_cont by auto
+
+
+
+  have Test : "\<And>P0 P1 ci c' x . 
+  (((\<forall> st . P0 st \<longrightarrow> P1 st) \<and> x = [G Swhile' [cond, body]] ) \<or>
+   ((\<forall> st . P0 st \<longrightarrow> P1 st) \<and> x = [cond, G Swhile' [cond, cond, body]]) \<or>
+   ( (\<forall> st . P0 st \<longrightarrow> P1 st \<and> get_cond st = Some True) \<and> x = [body, G Swhile' [cond, body]]) \<or>
+   ((\<forall> st . P0 st \<longrightarrow> P1 st \<and> get_cond st = Some False) \<and> x = []) ) \<Longrightarrow>
+  |gs| {-P1-} [cond] {-P1-} \<Longrightarrow>
+  |gs| {- (\<lambda> st . P1 st \<and> get_cond st = Some True) -} [body]
+                        {- P1 -} \<Longrightarrow>
+  |gs| {\<lambda> st . P1 st \<and> get_cond st = Some True} [body]  @ c' \<Longrightarrow>
+  (\<And> st . P1 st \<Longrightarrow> get_cond st \<noteq> None) \<Longrightarrow>
+  |gs| { P1 } [cond] @ c' \<Longrightarrow>
+  |gs| {P1} c' \<Longrightarrow>
+  (( |gs| {P0} (x @ c')))"
+  proof
+    fix P0 P1 :: "(bool md_triv option md_prio * int md_triv option md_prio * 'b) \<Rightarrow> bool" 
+    fix ci c' x
+    fix m :: "('a, 'b) state"
+
+    assume Pre : "(((\<forall> st . P0 st \<longrightarrow> P1 st) \<and> x = [G Swhile' [cond, body]] ) \<or>
+   ((\<forall> st . P0 st \<longrightarrow> P1 st) \<and> x = [cond, G Swhile' [cond, cond, body]]) \<or>
+   ( (\<forall> st . P0 st \<longrightarrow> P1 st \<and> (get_cond st) = Some True) \<and> x = [body, G Swhile' [cond, body]]) \<or>
+   ((\<forall> st . P0 st \<longrightarrow> P1 st \<and>  (get_cond st) = Some False) \<and> x = []) )"
+    assume Hcond : "|gs| {-P1-} [cond] {-P1-} "
+    assume Htrue : "|gs| {- (\<lambda> st . P1 st \<and> get_cond st = Some True) -} [body] {- P1 -} "
+    assume A0 : "|gs| {\<lambda> m . P1 m \<and> get_cond m = Some True} [body] @ c'"
+    assume A1 : "|gs| {P1} [cond] @ c'"
+    assume cndn : "|gs| {P1} c'"
+    assume Pay : "P0 (payload m)"
+    assume Cont : "s_cont m = Inl (x @ c') "
+
 
     show "safe gs m"
     proof
@@ -652,14 +1097,255 @@ proof
       obtain n where N: "sem_exec_c_p gs m n m'"
         using exec_p_imp_exec_c_p[OF Exc] by auto
 
-      show "imm_safe gs m'" using N A0 A1 Pay Cont unfolding sem_exec_p_def
-      proof(induction arbitrary: c'  rule: sem_exec_c_p.induct)
+      show "imm_safe gs m'" using Exc  Pre Hcond Htrue A0 A1 cndn Pay Cont unfolding sem_exec_p_def 
+      proof(induction arbitrary: x ci c' P1 P0 rule: converse_rtranclp_induct)
+        case base
+        then show ?case sorry
+      next
+        case (step y z)
+        consider (C1) "(\<forall> st . P0 st \<longrightarrow> P1 st) \<and> x = [G Swhile' [cond, body]]" |
+          (C2) "(\<forall> st . P0 st \<longrightarrow> P1 st) \<and> x = [cond, G Swhile' [cond, cond, body]]" |
+          (C3) "(\<forall> st . P0 st \<longrightarrow> P1 st \<and> (get_cond st) = Some False) \<and> x = []" |
+          (C4) "(\<forall> st . P0 st \<longrightarrow> P1 st \<and> (get_cond st) = Some True) \<and> x = [body, G Swhile' [cond, body]]"
+          using step.prems(1) by auto
+        then show ?thesis
+        proof cases
+          case C1
+
+          then have C1_1 : "(\<forall> st . P0 st \<longrightarrow> P1 st)" and C1_2 : "x = [G Swhile' [cond, body]]" by auto
+
+
+          obtain ci' where CI' : "s_cont z = Inl (ci')" using step.hyps step.prems
+            sorry
+
+          show ?thesis using step.IH 
+
+
+  have Test : "\<And>P0 P1 ci c' x . 
+  ( |gs| {-P0-} ci {-P1-} ) \<Longrightarrow>
+  (( |gs| {-P1-} ci {-P1-} \<and> x = [G Swhile' [cond, body]] ) \<or>
+   ( |gs| {-P1-} ci {- P1 -} \<and> x = [cond, G Swhile' [cond, cond, body]]) \<or>
+   ( |gs| {-P1-} ci {-(\<lambda> st . P1 st \<and> get_cond st = Some True) -} \<and> x = [body, G Swhile' [cond, body]]) \<or>
+   ( |gs| {-P1-} ci {-(\<lambda> st . P1 st \<and> get_cond st = Some False) -} \<and> x = []) ) \<Longrightarrow>
+  |gs| {-P1-} [cond] {-P1-} \<Longrightarrow>
+  |gs| {- (\<lambda> st . P1 st \<and> get_cond st = Some True) -} [body]
+                        {- P1 -} \<Longrightarrow>
+  |gs| {\<lambda> st . P1 st \<and> get_cond st = Some True} [body]  @ c' \<Longrightarrow>
+  (\<And> st . P1 st \<Longrightarrow> get_cond st \<noteq> None) \<Longrightarrow>
+  |gs| { P1 } [cond] @ c' \<Longrightarrow>
+  |gs| {P1} c' \<Longrightarrow>
+  (( |gs| {P0} (ci @ x @ c')))"
+  proof
+    fix P0 P1 ci c' x
+    fix m :: "('a, 'b) state"
+
+    assume Pre0 : "|gs| {-P0-} ci {-P1-} "
+    assume Pre : "(( |gs| {-P1-} ci {-P1-} \<and> x = [G Swhile' [cond, body]] ) \<or>
+   ( |gs| {-P1-} ci {- P1 -} \<and> x = [cond, G Swhile' [cond, cond, body]]) \<or>
+   ( |gs| {-P1-} ci {-(\<lambda> st . P1 st \<and> get_cond st = Some True) -} \<and> x = [body, G Swhile' [cond, body]]) \<or>
+   ( |gs| {-P1-} ci {-(\<lambda> st . P1 st \<and> get_cond st = Some False) -} \<and> x = []) )"
+    assume Hcond : "|gs| {-P1-} [cond] {-P1-} "
+    assume Htrue : "|gs| {- (\<lambda> st . P1 st \<and> get_cond st = Some True) -} [body] {- P1 -} "
+    assume A0 : "|gs| {\<lambda> m . P1 m \<and> get_cond m = Some True} [body] @ c'"
+    assume A1 : "|gs| {P1} [cond] @ c'"
+    assume cndn : "|gs| {P1} c'"
+    assume Pay : "P0 (payload m)"
+    assume Cont : "s_cont m = Inl (ci @ x @ c') "
+
+
+    show "safe gs m"
+    proof
+      fix m'
+      assume Exc : "sem_exec_p gs m m'"
+
+      obtain n where N: "sem_exec_c_p gs m n m'"
+        using exec_p_imp_exec_c_p[OF Exc] by auto
+
+      show "imm_safe gs m'" using Exc Pre0 Pre Hcond Htrue A0 A1 cndn Pay Cont unfolding sem_exec_p_def 
+      proof(induction arbitrary: x ci c' P1 P0 rule: converse_rtranclp_induct)
+        case base
+        then show ?case sorry
+      next
+        case (step y z)
+        consider (C1) "|gs| {-P1-} ci {-P1-} \<and> x = [G Swhile' [cond, body]]" |
+          (C2) "|gs| {-P1-} ci {-\<lambda>st. P1 st-} \<and> x = [cond, G Swhile' [cond, cond, body]]" |
+          (C3) "|gs| {-P1-} ci {-\<lambda>st. P1 st \<and> get_cond st = Some False-} \<and> x = []" |
+          (C4) "|gs| {-P1-} ci {-\<lambda>st. P1 st \<and> get_cond st = Some True-} \<and> x = [body, G Swhile' [cond, body]]"
+          using step.prems(2) by auto
+        then show ?thesis
+        proof cases
+          case C1
+
+          then have C1_1 : "|gs| {-P1-} ci {-P1-}" and C1_2 : "x = [G Swhile' [cond, body]]" by auto
+
+          have C1_1' : "|gs| {- P1 -} ci @ [cond] {- P1 -}"
+            using HCat[OF C1_1 step.prems(3)] by auto
+
+          obtain ci' where CI' : "s_cont z = Inl (ci')" using step.hyps step.prems
+            sorry
+
+          obtain ci' where CI' : "s_cont z = Inl (ci')" using step.hyps step.prems
+            sorry
+(* ci1? *)
+
+(* if we can get this we are done. *)
+          have CI0 : "|gs| {P1} x @ c'" 
+          proof
+            fix m00 :: "('a, 'b) state"
+            assume P00 : "P1 (payload m00)"
+
+            assume "s_cont m00 = Inl (x @ c')"
+
+            obtain m01 where "sem_step_p gs m00 m01" sorry
+
+            have Z : "s_cont m01 = Inl (cond # G Swhile' [cond, cond, body] # c')"
+              sorry
+
+            have Yp : "P1 (payload m01)" sorry
+
+
+            have 1 : "|gs| {-P1-} ci {-P1-} \<and> [cond, G Swhile' [cond, cond, body]] = [G Swhile' [cond, body]] \<or>
+  |gs| {-P1-} ci {-P1-} \<and> [cond, G Swhile' [cond, cond, body]] = [cond, G Swhile' [cond, cond, body]] \<or>
+  |gs| {-P1-} ci {-\<lambda>st. P1 st \<and> get_cond st = Some True-} \<and> [cond, G Swhile' [cond, cond, body]] = [body, G Swhile' [cond, body]] \<or>
+  |gs| {-P1-} ci {-\<lambda>st. P1 st \<and> get_cond st = Some False-} \<and> [cond, G Swhile' [cond, cond, body]] = []"
+              using C1 step.prems by auto
+
+              show "safe gs m00" using step.IH[OF C1_1 1] 
+                using Z unfolding Nil by auto
+
+
+
+            have X: "|gs| {P0} (ci @ x @ c')" using HTE[OF step.prems(1) CI0] by auto
+  
+            have sf : "safe gs y" using guardedD[OF X `P0 (payload y)` `s_cont y = Inl (ci @ x @ c')`]
+              by auto
+  
+            have xc : "sem_exec_p gs y m'" using 
+                step.hyps unfolding sem_exec_p_def
+              by auto
+  
+
+          show ?thesis using safeD[OF sf xc] by auto
+
+(* can we merge these cases? *)
+          show ?thesis 
+          proof(cases ci)
+            case Nil
+
+            have Ci : "|gs| {- P0 -} [] {- P1 -}"
+              using step unfolding Nil by auto
+
+            have Z : "s_cont z = Inl (cond # G Swhile' [cond, cond, body] # c')"
+              sorry
+
+(*
+            then have Z' : "s_cont z = Inl ((ci @ [cond]) @ [x] @ c')"
+              using Nil C1_2 by auto
+*)
+            have Yp : "P1 (payload y)" sorry
+
+            have Zp : "P1 (payload z)" sorry
+
+
+            have 1 : "|gs| {-P1-} ci {-P1-} \<and> [cond, G Swhile' [cond, cond, body]] = [G Swhile' [cond, body]] \<or>
+  |gs| {-P1-} ci {-P1-} \<and> [cond, G Swhile' [cond, cond, body]] = [cond, G Swhile' [cond, cond, body]] \<or>
+  |gs| {-P1-} ci {-\<lambda>st. P1 st \<and> get_cond st = Some True-} \<and> [cond, G Swhile' [cond, cond, body]] = [body, G Swhile' [cond, body]] \<or>
+  |gs| {-P1-} ci {-\<lambda>st. P1 st \<and> get_cond st = Some False-} \<and> [cond, G Swhile' [cond, cond, body]] = []"
+              using C1 step.prems by auto
+        
+
+            show ?thesis using step.IH[OF C1_1 1 step.prems(3) step.prems(4) step.prems(5) step.prems(6) step.prems(7) Zp] 
+              using Z unfolding Nil by auto
+
+          next
+            case (Cons ci1 cis)
+
+            obtain ci' where CI' : "s_cont z = Inl (ci')" using step.hyps step.prems
+              sorry
+(* ci1? *)
+
+            have CI0 : "|gs| {P1} x @ c'" sorry
+
+            have X: "|gs| {P0} (ci @ x @ c')" using HTE[OF step.prems(1) CI0] by auto
+
+            have sf : "safe gs y" using guardedD[OF X `P0 (payload y)` `s_cont y = Inl (ci @ x @ c')`]
+              by auto
+
+            have xc : "sem_exec_p gs y m'" using 
+                step.hyps unfolding sem_exec_p_def
+              by auto
+
+            show ?thesis using safeD[OF sf xc] by auto
+
+            show ?thesis using guardedD[OF X `P0 (payload y)` ]
+
+            show ?thesis using HTE[OF step.prems(1) guard_emp]
+
+            have "|gs| { (\<lambda> st . st = payload z) } ci'"
+            proof
+              fix my :: "('a, 'b) state"
+
+              assume "payload my = payload z"
+(*
+              then obtain sty where Sty : "sem_step_p gs z sty" and Styp : "payload sty = payload my"
+                by auto
+*)
+              assume "s_cont my = Inl (ci')"
+
+
+              show "safe gs my" using step
+
+(* ok - is the issue that we can crash based on syntax and this isn't captured in our Hoare predicates? *)
+                show "safe gs my"
+                  using step.hyps HTE[OF step.prems(1), of "[]"]
+
+
+            then show ?thesis using
+                step.IH[OF step.prems(1)] step.prems(1)
+
+
+
+          next
+            case (Cons a list)
+            then show ?thesis sorry
+          qed
+        next
+          case C2
+          then show ?thesis sorry
+        qed
+      qed
+(*
+        apply(drule_tac rtranclp_induct_alt)
+          apply(auto simp only:)
+           defer (* safe because either ci is nonempty and ci steps, or else we are at while, which is safe for 1 step *)
+           defer
+*)
+
+
+      proof(induction  rule: rtranclp_induct_alt)
+        case 1
+        then show ?thesis sorry
+      next
+        case 2
+        then show ?thesis sorry
+      next
+        case (3 y z)
+        then show ?case sorry
+      qed
+        case base
+        then show ?case sorry
+      next
+        case (step y z)
+        then show ?case 
+      qed
+
+      proof(induction arbitrary: ci x c'  rule: sem_exec_c_p.induct)
         case (Excp_0 mx)
         then show ?case 
         proof(cases "sem_step gs mx")
           case (Inr bad)
-          then have False using Excp_0
-            by(auto simp add: sem_step_def)
+          then have False using Excp_0 HTE[OF Excp_0.prems(1)]
+            by(cases c0; auto simp add: sem_step_def)
           thus ?thesis by auto
         next
           case (Inl m')
@@ -684,7 +1370,83 @@ proof
         proof(cases "sem_step gs m1")
           case (Inr bad)
           then have False using Excp_Suc
-            by(auto simp add: sem_step_def)
+            by(cases c0; auto simp add: sem_step_def)
+          thus ?thesis by auto
+        next
+          case (Inl m1')
+
+          consider (C1) "|gs| {-P1-} ci {-P1-} \<and> x = G Swhile' [cond, body]" |
+            (C2) "|gs| {-P1-} ci {-\<lambda>st. P1 st \<and> get_cond st = Some True-} \<and> x = G Swhile' [cond, cond, body]"
+            using Excp_Suc.prems(1) by auto
+          then show ?thesis
+          proof cases
+            case C1
+
+            then have C1_1 : "|gs| {-P1-} ci {-P1-}" by auto
+            then show ?thesis 
+              using Excp_Suc.IH Excp_Suc.prems Excp_Suc.hyps HTE[OF C1_1 ]
+          next
+            case C2
+            then show ?thesis sorry
+          qed
+
+(*
+  have Test : "\<And> c0 c' . |gs| {-P1-} c0 {-P1-} \<Longrightarrow>
+|gs| {\<lambda> st . P1 st \<and> get_cond st = Some True}  [body, G Swhile' [cond, body]]  @ c' \<Longrightarrow>
+|gs| { P1 } [cond, G Swhile' [cond, cond, body]] @ c' \<Longrightarrow>
+|gs| {P1} (c0 @ [G Swhile' [cond, body]] @ c')"
+  proof
+    fix c0 c' 
+    fix m :: "('a, 'b) state"
+
+    assume A00 : "|gs| {-P1-} c0 {-P1-}"
+    assume A0 : "|gs| {\<lambda> m . P1 m \<and> get_cond m = Some True} [body, G Swhile' [cond, body]] @ c'"
+    assume A1 : "|gs| {P1} [cond, G Swhile' [cond, cond, body]] @ c'"
+    assume Pay : "P1 (payload m)"
+    assume Cont : "s_cont m = 
+      Inl (c0 @ [G Swhile' [cond, body]] @ c')"
+
+    show "safe gs m"
+    proof
+      fix m'
+      assume Exc : "sem_exec_p gs m m'"
+
+      obtain n where N: "sem_exec_c_p gs m n m'"
+        using exec_p_imp_exec_c_p[OF Exc] by auto
+
+      show "imm_safe gs m'" using N A00 A0 A1 Pay Cont unfolding sem_exec_p_def
+      proof(induction arbitrary: c0 c'  rule: sem_exec_c_p.induct)
+        case (Excp_0 mx)
+        then show ?case 
+        proof(cases "sem_step gs mx")
+          case (Inr bad)
+          then have False using Excp_0 HTE[OF Excp_0.prems(1)]
+            by(cases c0; auto simp add: sem_step_def)
+          thus ?thesis by auto
+        next
+          case (Inl m')
+
+          have F_eq : "sem_step \<lparr> s_sem = f \<rparr> mx = Inl m'"
+            using sym[OF dominant_pcomps'[OF Hpres Hnemp Hdom]] Excp_0 Inl H0
+            by(simp add: sem_step_def)
+
+          have "sem_step gs mx = Inl m'" 
+            using Hsyn H0 F_eq Inl unfolding HF
+            by(cases m'; auto simp add: s_cont_def sem_step_def imp_sem_l_gen_def imp_ctl_sem_def imp_sem_lifting_gen_def
+           schem_lift_defs 
+            merge_l_def fst_l_def snd_l_def prio_l_def triv_l_def option_l_def LNew_def
+            split: md_prio.splits md_triv.splits option.splits)
+
+          thus ?thesis
+            unfolding imm_safe_def sem_step_p_eq by blast
+        qed
+      next
+        case (Excp_Suc m1 m2 n m3)
+        then show ?case 
+        proof(cases "sem_step gs m1")
+          case (Inr bad)
+          then have False using Excp_Suc
+            by(cases c0; auto simp add: sem_step_def)
           thus ?thesis by auto
         next
           case (Inl m1')
@@ -719,7 +1481,7 @@ proof
                 split: md_prio.splits md_triv.splits option.splits)
 
           show ?thesis
-            using Excp_Suc.IH[OF Excp_Suc.prems(1) ]  Excp_Suc.prems
+            using Excp_Suc.IH  Excp_Suc.prems
 
           proof(cases "sem_step gs m1'")
             case Inr' : (Inr bad)
@@ -1002,6 +1764,6 @@ proof
 qed
 qed
 
-
+*)
 
 end
